generic/GenericSoundness.ec
@@ -2,7 +2,7 @@ pragma Goals:printall.
 require import AllCore List Distr.
 
 require GenericCompleteness.
-clone include GenericCompleteness. (* inherit defs. from GenericCompleteness *)
+clone include GenericCompleteness. (* inherit defs.  *)
 
 op soundness_relation : relation.
 
@@ -10,7 +10,6 @@ module type MaliciousProver = {
   proc commitment(s: statement) : commitment
   proc response(challenge: challenge) : response
 }.
-
 
 module Soundness(P: MaliciousProver, V: HonestVerifier) = {
   proc run(statement: statement) : bool = {
@@ -46,11 +45,11 @@ clone import WhileNotBProc as WNBP with type rt <- bool,
 
 section.
 
-declare module P <: MaliciousProver {-M, -HonestVerifier}.
+declare module P <: MaliciousProver {-M, -HV}.
 
 (* are these needed? after all we are proving <= probability *)
-declare axiom verify_ll : islossless HonestVerifier.verify.
-declare axiom challenge_ll : islossless HonestVerifier.challenge.
+declare axiom verify_ll : islossless HV.verify.
+declare axiom challenge_ll : islossless HV.challenge.
 declare axiom response_ll : islossless P.response.
 declare axiom commitment_ll : islossless P.commitment.
 
@@ -58,33 +57,33 @@ op deltoid : real.
 
 declare axiom soundness &n statement:
     ! in_language soundness_relation statement =>
-     Pr[Soundness(P, HonestVerifier).run(statement) @ &n : res]
-        <= deltoid.
+     Pr[Soundness(P,HV).run(statement) @ &n : res]
+         <= deltoid.
 
 lemma soundness_seq &m statement n:
     ! in_language soundness_relation statement =>
      0 <= n =>
-     Pr[SoundnessAmp(P, HonestVerifier).run(statement, n) @ &m : res]
-     <= deltoid ^ (n + 1).
+     Pr[SoundnessAmp(P,HV).run(statement, n) @ &m : res]
+       <= deltoid ^ (n + 1).
 proof.
 move => nil nz.
-have phs : phoare[ Soundness(P,HonestVerifier).run : arg = (statement) ==> res ] <= deltoid.
+have phs : phoare[ Soundness(P,HV).run : arg = (statement) ==> res ] <= deltoid.
 bypr. move => &m0 H. 
 rewrite H. simplify. apply soundness.  assumption.
-have ->: Pr[SoundnessAmp(P, HonestVerifier).run(statement, n) @ &m : res]    
- = Pr[ M(Soundness(P,HonestVerifier)).whp((statement), fun x => !x,1,n+1, true) @ &m :  res ].
-byequiv (_: ={glob P, glob HonestVerifier} /\  arg{1} = (statement, n) /\ arg{2} = ((statement), fun x => !x,1,n+1, true)  ==> _).  
+have ->: Pr[SoundnessAmp(P, HV).run(statement, n) @ &m : res]    
+ = Pr[ M(Soundness(P,HV)).whp((statement), fun x => !x,1,n+1, true) @ &m :  res ].
+byequiv (_: ={glob P, glob HV} /\  arg{1} = (statement, n) /\ arg{2} = ((statement), fun x => !x,1,n+1, true)  ==> _).  
 proc.   sp.
-while (i{1} + 1 = M.c{2} /\ N{1} + 1 = e{2} /\ accept{1} = !MyP{2} r{2} /\ ={glob P, glob HonestVerifier}
+while (i{1} + 1 = M.c{2} /\ N{1} + 1 = e{2} /\ accept{1} = !MyP{2} r{2} /\ ={glob P, glob HV}
   /\ (i{2}, MyP{2}, s{2}, e{2}) =
   ((stat{1}), fun (x : bool) => !x, 1, N{1}+1)  ).
-wp.  call (_: ={glob P, glob HonestVerifier}).
+wp.  call (_: ={glob P, glob HV}).
 sim. skip. progress. smt. smt.
 skip. progress.  smt. smt.
 auto.  auto.
 byphoare (_: arg = ((statement), fun (x : bool) => !x,
                                        1, n + 1, true) ==> _).
-apply (asdsadq_le (Soundness(P,HonestVerifier))). 
+apply (asdsadq_le (Soundness(P,HV))). 
 proc.
 call verify_ll. call response_ll. call challenge_ll. call commitment_ll. skip. auto.
 apply phs. auto. 
